code/experimental/SPARKLE/Hacl.Impl.Sparkle.fst
@@ -24,7 +24,6 @@ let rcon_buffer: x: glbuffer uint32 vsize_rcon
   createL_global rcon_list
 
 
-
 type branch_len =  n: size_t {v n = 1 \/ v n = 2 \/ v n = 3 \/ v n = 4 \/ v n = 6 \/ v n = 8}
 
 type branch branch_len = lbuffer uint32 (2ul *! branch_len)
@@ -62,12 +61,23 @@ let l1 x = (x <<<. size 16)  ^. (x &. (u32 0xffff))
 
 
 inline_for_extraction noextract
-val getBranchI: #l: branch_len -> b: branch l -> i: size_t {v i < v l / 2} -> 
+val getBranch: #l: branch_len -> b: branch l -> i: size_t {v i < v l / 2} -> 
   Stack (tuple2 uint32 uint32)
   (requires fun h -> live h b)
   (ensures fun h0 _ h1 -> modifies0 h0 h1)
 
-let getBranchI #l b i =  Lib.Buffer.index b i, Lib.Buffer.index b (i +! 1ul)
+let getBranch #l b i =  Lib.Buffer.index b i, Lib.Buffer.index b (i +! 1ul)
+
+
+inline_for_extraction noextract 
+val setBranch: #n: branch_len -> i: size_t {v i < v n / 2} -> branch1 -> b: branch n -> 
+  Stack unit 
+  (requires fun h -> live h b)
+  (ensures fun h0 _ h1 -> modifies (loc b) h0 h1)  
+
+let setBranch #n i (x, y) b =
+  upd #uint32 b (2ul *. i) x;
+  upd #uint32 b (2ul *. i +. 1ul) y
 
 
 inline_for_extraction noextract
@@ -80,7 +90,7 @@ val xor_step: #l: branch_len -> b: branch l
     (ensures fun h0 _ h1 -> modifies (loc tx |+| loc ty) h0 h1)
 
 let xor_step #l b tx ty i = 
-  let xi, yi = getBranchI b i in 
+  let xi, yi = getBranch b i in 
   let tx_0 = index tx (size 0) in 
   let ty_0 = index ty (size 0) in 
   upd tx (size 0) (xi ^. tx_0);
@@ -98,12 +108,31 @@ let xor #l b =
     let tu = create (size 1) (u32 0) in  
   Lib.Loops.for 0ul (l >>. 1ul) 
     (fun h i ->live h b /\ live h tu /\ live h tx /\ disjoint tx tu /\ modifies (loc tx |+| loc tu) h0 h) 
-    (fun (i: size_t {v i < v l / 2}) -> 
-      let h = ST.get() in 
-      xor_step b tx tu i);
+    (fun (i: size_t {v i < v l / 2}) -> xor_step b tx tu i);
 
   let u = index #MUT #_ #1ul tx (size 0) in 
   let v = index #MUT #_ #1ul tu (size 0) in 
   pop_frame(); 
   (u, v)
     
+
+inline_for_extraction noextract
+val xor_x_step: #l: branch_len -> b: branch l -> lty: uint32 -> ltx: uint32 -> i: size_t {v i < v l / 2} -> 
+  Stack unit 
+    (requires fun h -> live h b)
+    (ensures fun h0 _ h1 -> modifies (loc b) h0 h1)
+
+let xor_x_step #l b lty ltx i = 
+  let xi, yi = getBranch #l b i in 
+  let xi_n, yi_n = xi ^. lty, yi ^. ltx in
+  setBranch i (xi_n, yi_n) b
+
+
+val xor_x: #l: branch_len -> b: branch l -> lty: uint32 -> ltx: uint32 -> Stack unit 
+  (requires fun h -> live h b)
+  (ensures fun h0 _ h1 -> True)
+  
+let xor_x #l b lty ltx = 
+  Lib.Loops.for (0ul) (l >>. 1ul)  (fun h i -> live h b) (fun (i: size_t {v i < v l / 2})  -> xor_x_step b lty ltx i)
+
+
